michael_formal/EFSM_LTL.thy
@@ -5,7 +5,7 @@ begin
 definition step :: "efsm \<Rightarrow> statename \<Rightarrow> registers \<Rightarrow> label \<Rightarrow> inputs \<Rightarrow> (statename \<times> outputs \<times> registers)" where
 "step e s r l i \<equiv>
   case (possible_steps e s r l i) of
-    [(s',t)] \<Rightarrow> (s', (apply_outputs (Outputs t) (join_ir i r 1)), (apply_updates (Updates t) (join_ir i r 1) r)) |
+    [(s',t)] \<Rightarrow> (s', (apply_outputs (Outputs t) (join_ir i r)), (apply_updates (Updates t) (join_ir i r) r)) |
     _ \<Rightarrow> (0, [], r)"
 
 abbreviation neXt :: "efsm \<Rightarrow> statename \<Rightarrow> registers \<Rightarrow> event \<Rightarrow> ((statename \<times> outputs \<times> registers) \<Rightarrow> event \<Rightarrow> bool) \<Rightarrow> bool" where
@@ -25,17 +25,17 @@ G(
   );
 *)
 
-lemma read_not_none [simp]: "\<forall>r'. step filesystem 2 r ''read'' [] \<noteq> (0, [], r')"
+lemma read_not_none : "\<forall>r'. step filesystem 2 r ''read'' [] \<noteq> (0, [], r')"
   by (simp add: fs_simp step_def)
 
-lemma read_no_side_effects [simp]: "\<exists>p. step filesystem 2 r ''read'' [] = (2, p, r)"
+lemma read_no_side_effects : "\<exists>p. step filesystem 2 r ''read'' [] = (2, p, r)"
   apply (simp add: fs_simp step_def)
   apply (case_tac "r ''r1'' = r ''r3''")
    apply simp
   apply (rule ext)
   by auto
 
-lemma read_no_side_effects2 [simp]: "step filesystem 2 r ''read'' [] = a \<Longrightarrow> snd (snd a) = r \<and> fst a = 2"
+lemma read_no_side_effects2 : "step filesystem 2 r ''read'' [] = a \<Longrightarrow> snd (snd a) = r \<and> fst a = 2"
   apply (simp add: step_def)
   apply (simp add: fs_simp)
   apply (case_tac "r ''r1'' = r ''r3''")
@@ -69,19 +69,51 @@ lemma read_denied1: "r ''r1'' \<noteq> r ''r3'' \<Longrightarrow> EFSM_LTL.step 
   apply (simp add: fs_simp step_def)
   by (rule ext, simp)
 
-lemma aux1: "r ''r1'' = r ''r3'' \<Longrightarrow>
-    (\<lambda>x. if x = ''r1'' then aval (snd (''r1'', V ''r1'')) r else apply_updates [(''r2'', V ''r2''), (''r3'', V ''r3'')] r r x) = r"
-  by (rule ext, simp)
-
 lemma read_step: "EFSM_LTL.step filesystem 2 r ''read'' [] = (2, [r ''r2''], r) \<or>
 EFSM_LTL.step filesystem 2 r ''read'' [] = (2, [0], r)"
   apply (case_tac "r ''r1'' = r ''r3''")
    apply (simp add: read_success)
   by (simp add: read_denied1)
 
-lemma "all (t) (\<lambda>e. e = (''read'', []) \<or> e = (''logout'', []) \<or> (fst e = ''write'' \<and> length (snd e) = 1)) \<Longrightarrow> 
- \<forall> outs r. globally filesystem (2, outs, r) t (\<lambda>s e r' p. (s = 2 \<and> fst e = ''write'' \<and> r' ''r1'' = 1) \<longrightarrow>
-  globally filesystem (2, outs, r) t (\<lambda>s e r' p. (s = 2 \<and> fst e = ''read'' \<and> r' ''r1'' \<noteq> 1)) \<longrightarrow>
+lemma logout: "(EFSM_LTL.step filesystem 2 r ''logout'' []) = (1, [], r)"
+  apply (simp add: fs_simp step_def)
+  by (rule ext, simp)
+
+lemma login_2: "fst a = ''login'' \<Longrightarrow> EFSM_LTL.step filesystem 2 r (fst a) (snd a) = (0, [], r)"
+  by (simp add: fs_simp step_def)
+
+lemma index2state_i1: "length (snd a) = Suc 0 \<Longrightarrow> index2state (snd a) 1 ''i1'' = hd (snd a)"
+  by (metis Suc_length_conv i1 index2state.simps(2) list.sel(1))
+
+lemma writes: "fst a = ''write'' \<and> length (snd a) = Suc 0 \<Longrightarrow>
+                r ''r1'' \<noteq> r ''r3'' \<Longrightarrow> 
+                EFSM_LTL.step filesystem 2 r ''write'' (snd a) = (2, [], (\<lambda>x. if x = ''r2'' then hd (snd a) else (if x = ''r3'' then r ''r1'' else r x)))"
+  apply (simp add: fs_simp step_def)
+  apply safe
+  apply (rule ext)
+  apply simp
+  by (simp add: index2state_i1)
+
+lemma nomoreinputs: "a \<noteq> (''read'', []) \<Longrightarrow>
+         a \<noteq> (''logout'', []) \<Longrightarrow>
+         fst a \<noteq> ''write'' \<Longrightarrow>
+         (EFSM_LTL.step filesystem 2 r (fst a) (snd a)) = (0, [],r)"
+  apply (simp add: fs_simp step_def)
+  by (metis prod.collapse)
+
+lemma dead_state: "globally filesystem (0, [], r) t (\<lambda>s e r' p. s \<noteq> 0) \<Longrightarrow> False"
+proof (induction t)
+case Nil
+  then show ?case by simp
+next
+  case (Cons a t)
+  then show ?case by simp
+qed
+
+lemma "all (t) (\<lambda>e. e = (''read'', []) \<or> e = (''login'', []) \<or> e = (''logout'', []) \<or> (fst e = ''write'' \<and> length (snd e) = 1)) \<Longrightarrow>
+ \<forall> outs r. globally filesystem (state, outs, r) t (\<lambda>s e r' p. s \<noteq> 0) \<longrightarrow>
+globally filesystem (state, outs, r) t (\<lambda>s e r' p. (s = 2 \<and> fst e = ''write'' \<and> r' ''r1'' = 1) \<longrightarrow>
+  globally filesystem (state, outs, r) t (\<lambda>s e r' p. (s = 2 \<and> fst e = ''read'' \<and> r' ''r1'' \<noteq> 1)) \<longrightarrow>
     neXt filesystem s' r'' (hd t') (\<lambda>spr e. (fst (snd spr)) = [0])
 )"
 proof (induction t)
@@ -90,38 +122,46 @@ proof (induction t)
 next
   case (Cons a t')
   then show ?case
-    apply (case_tac "a = (''read'', [])", simp)
-     apply (rule allI)
-     apply (case_tac "(EFSM_LTL.step filesystem 2 r ''read'' []) = (2, [0], r)", simp)
+    apply (case_tac "state = 2")
+     apply (case_tac "a = (''read'', [])", simp)
+      apply (rule allI)
+      apply (case_tac "(EFSM_LTL.step filesystem 2 r ''read'' []) = (2, [0], r)", simp)
+       apply (case_tac "r ''r1'' = 1")
+        apply (simp add: truefun)
+       apply simp
       apply (case_tac "r ''r1'' = 1")
        apply (simp add: truefun)
       apply simp
-     apply (case_tac "r ''r1'' = 1")
-      apply (simp add: truefun)
+      apply (case_tac "r ''r3'' = 1")
+       apply (simp add: read_denied)
+      apply (case_tac "r ''r1'' = r ''r3''")
+       apply (simp add: read_success)
+      apply (simp add: read_denied1)
+
+     apply (case_tac "fst a = ''write'' \<and> length (snd a) = 1", simp)
+      apply (frule allI)
+      apply (case_tac "r ''r1'' = r ''r3''")
+    using truefun apply blast
+      apply (simp add: writes truefun)
+
+    apply (case_tac "a = (''logout'', [])", simp)
+    apply (simp add: logout truefun)
+
+     apply (rule allI, rule allI)
+     apply safe
+      apply (simp add: nomoreinputs)
+      apply (metis (no_types, lifting) dead_state fst_conv login_2)
+
      apply simp
-     apply (case_tac "r ''r3'' = 1")
-      apply (simp add: read_denied)
-    apply (case_tac "r ''r1'' = r ''r3''")
-      apply (simp add: read_success)
-     apply (simp add: read_denied1)
+     apply (metis (no_types, lifting) dead_state fst_conv login_2)
 
-     
-    
+    apply (case_tac "state = 0")
+     apply simp
 
-
-
-     
-
-
+    apply (case_tac "state = 1")
+     apply (case_tac "fst a = ''login'' \<and> length (snd a) = 1")
+      apply (simp add: truefun)
+     apply (simp add: truefun)
+    by (simp add: truefun)
 qed
-
-
-
-
-
-
-
-    
-qed
-
 end
